Addressing code review comments.

Coq/EC/GeneratorMul.v
@@ -115,6 +115,8 @@ Section GeneratorMulWNAF.
     OddWindow w ->
     pExpMultiple n w == groupMul_doubleAdd_signed (Z.shiftl w (Z.of_nat (numPrecompExponentGroups * wsize * n))) p.
 
+  (* An alternative semantics for double/add operations that perform all additions by a table lookup. If the required value is not
+  in the table, then the operation fails. *)
   Definition evalWindowMult_precomp(p : GroupElem) (m : WindowedMultOp) (e : GroupElem) :=
   match m with
   | wm_Add n w => 
@@ -122,6 +124,7 @@ Section GeneratorMulWNAF.
   | wm_Double n => Some (groupDouble_n (n * wsize) e)
   end.
 
+  (* Evaluate a double/add program using table lookups of addition operations. *)
   Fixpoint groupMul_signedWindows_precomp (e : GroupElem)(ws : list WindowedMultOp) : option GroupElem :=
     match ws with
     | nil => Some e
@@ -132,6 +135,13 @@ Section GeneratorMulWNAF.
       end
     end.
 
+  (* Convert a simple windowed multiplication by permuting the addition operations and inserting doublings in a specific way. Then 
+  run the double/add program using the semantics that performs all add operations by table lookup. This will only succeed 
+  if doublings were inserted in a way that ensures all the add operations can be performed by table lookups. For example,
+  we can permute the numbers [0, 1, 2, 3, ...] (describing the position of each window) to get [0, 4, 8, ..., 1, 5, 9, ..., 2, 6, 10, ....]
+  and then insert a doubling after each part to decrease the following values by 1. This will result in a list where additions have 
+  exponents that look like [0, 4, 8, ..., 0, 4, 8, ..., 0, 4, 8, ...]. These additions can be calculated using table lookups into a table
+  that only includes multiples of 2^0, 2^4, 2^8, etc. *)
   Definition groupedMul_precomp d ws :=
     match (permuteAndDouble ws d (flatten (groupIndices numWindows numPrecompExponentGroups)) (endIndices (groupIndices numWindows numPrecompExponentGroups))) with
     | None => None
@@ -571,51 +581,6 @@ Section GeneratorMulWNAF.
     apply combineOpt_length in H.
     rewrite map_length in *.
     lia.
-
-  Qed.
-
-  Definition groupMul := groupMul groupAdd idElem.
-  Definition preCompTable := preCompTable groupAdd idElem groupDouble wsize.  
-
-  Hint Resolve groupMul_proper : typeclass_instances.
-
-  Fixpoint basePreCompTable m x n :=
-    match n with
-    | 0%nat => nil
-    | S n' => (preCompTable x) :: (basePreCompTable m (groupDouble_n m x) n')
-    end.
-
-  Theorem basePreCompTable_correct : forall n m x n1 n2,
-    (n1 < n)%nat ->
-    (n2 < Nat.pow 2 (pred wsize))%nat-> 
-    (List.nth n2 (List.nth n1 (basePreCompTable m x n) List.nil) idElem) == (groupMul ((2 * n2 + 1) * (Nat.pow 2 (n1 * m))) x).
-
-    induction n; destruct n1; intros; simpl in *; try lia.
-    unfold preCompTable.
-    erewrite preCompTable_nth; eauto.
-    simpl.
-    repeat rewrite plus_0_r.
-    repeat rewrite Nat.mul_1_r.
-    reflexivity.
-    unfold tableSize.
-    rewrite Nat.shiftl_1_l.
-    rewrite Nat.sub_1_r.
-    trivial.
-
-    erewrite IHn.
-    repeat rewrite plus_0_r.
-    unfold groupMul.
-    rewrite groupMul_assoc; eauto.
-    rewrite groupMul_assoc; eauto.
-    apply groupMul_proper; eauto.
-    unfold groupDouble_n.
-    rewrite groupDouble_n_groupMul_equiv; eauto.
-    rewrite plus_comm.
-    rewrite Nat.pow_add_r.
-    rewrite groupMul_assoc; eauto.
-    reflexivity.
-    lia.
-    trivial.
 
   Qed.
 
